Set up the necessary cheats for compute_add_thm

candle/prover/compute/computeScript.sml
@@ -2,8 +2,8 @@
   Implementation of the compute primitive.
  *)
 
-open preamble holSyntaxTheory holKernelTheory holKernelProofTheory
-     ml_monadBaseTheory;
+open preamble holSyntaxTheory holSyntaxExtraTheory holKernelTheory
+     holKernelProofTheory ml_monadBaseTheory;
 open computeSyntaxTheory;
 
 val _ = new_theory "compute";
@@ -30,12 +30,12 @@ Overload handle[local] = “handle_Failure”;
 Definition dest_num_def:
   dest_num tm =
     case tm of
-      Const n t => if n = «_0» then SOME 0 else NONE
+      Const n t => if tm = _0 then SOME 0 else NONE
     | Comb (Const nm t) r =>
         (case dest_num r of
         | NONE => NONE
-        | SOME n => if nm = «BIT0» then SOME (2 * n)
-                    else if nm = «BIT1» then SOME (2 * n + 1)
+        | SOME n => if Const nm t = _BIT0_TM then SOME (2 * n)
+                    else if Const nm t = _BIT1_TM then SOME (2 * n + 1)
                     else NONE)
     | _ => NONE
 End
@@ -44,7 +44,7 @@ Definition dest_numeral_def:
   dest_numeral tm =
     case tm of
       Comb (Const n t) r =>
-        if n = «NUMERAL» then
+        if Const n t = _NUMERAL_TM then
           case dest_num r of
           | NONE => raise_Failure «dest_numeral»
           | SOME n => st_ex_return n
@@ -57,6 +57,7 @@ Definition num_thms_def:
   num_thms = MAP (Sequent []) [
     (* T_DEF      *) _T === (Abs _X _X === Abs _X _X);
     (* FORALL_DEF *) _FORALL_TM === Abs _P (_P === Abs _X _T);
+    (* NUMERAL    *) _NUMERAL _N === _N;
     (* BIT0       *) _BIT0 _N === _ADD _N _N;
     (* BIT1       *) _BIT1 _N === _SUC (_ADD _N _N);
     (* ADD        *) _ADD _0 _M === _M;
@@ -67,18 +68,14 @@ End
 Theorem num_thms = SIMP_RULE list_ss [] num_thms_def;
 
 Definition init_def:
-  init ths =
-    case ths of
-      [] => T
-    | h::t => EXISTS (aconv (concl h) o concl) num_thms ∧
-              init t
+  init ths = EVERY (λth. MEM th ths) num_thms
 End
 
 Definition dest_binary_def:
-  dest_binary nm tm =
+  dest_binary tm' tm =
     case tm of
       Comb (Comb (Const n t) l) r =>
-        if n = nm then return (l, r)
+        if tm' = Const n t then return (l, r)
         else failwith «dest_binary»
     | _ => failwith «dest_binary»
 End
@@ -86,47 +83,115 @@ End
 Definition compute_add_def:
   compute_add ths tm =
     if ¬ (init ths) then failwith «compute_add: no init» else
-    do (l,r) <- dest_binary «+» tm;
+    do (l,r) <- dest_binary _ADD_TM tm;
        x <- dest_numeral l;
        y <- dest_numeral r;
        res <<- num2bit (x + y);
-       c <- mk_eq (tm,res);
+       c <- mk_eq (tm,_NUMERAL res);
        return (Sequent [] c)
     od ++ failwith «compute_add»
 End
 
 Theorem dest_binary_thm:
   STATE ctxt s ∧
-  TERM ctxt tm ⇒
-  dest_binary nm tm s = (res,s') ⇒
+  TERM ctxt tm ∧
+  TERM ctxt tm' ⇒
+  dest_binary tm' tm s = (res,s') ⇒
     s' = s ∧
     ∀l r. res = M_success (l,r) ⇒
-          TERM ctxt l ∧ TERM ctxt r
+          TERM ctxt l ∧ TERM ctxt r ∧
+          tm = Comb (Comb tm' l) r
 Proof
-  rw [dest_binary_def, raise_Failure_def, st_ex_return_def]
-  \\ every_case_tac \\ gs []
-  \\ gs [TERM_def, term_ok_def]
+  simp [dest_binary_def, raise_Failure_def, st_ex_return_def]
+  \\ strip_tac
+  \\ rpt CASE_TAC \\ gs []
+  \\ rw [] \\ gs [TERM_def, term_ok_def]
 QED
 
 Theorem dest_numeral_thm:
   STATE ctxt s ∧
   TERM ctxt tm ⇒
   dest_numeral tm s = (res,s') ⇒
-    s' = s
+    s' = s ∧
+    ∀n. res = M_success n ⇒
+        (numeral_thy_ok (thyof ctxt) ⇒ typeof tm = num_ty) ∧
+        ∃tm'. tm = _NUMERAL tm' ∧ dest_num tm' = SOME n
 Proof
-  rw [dest_numeral_def, raise_Failure_def, st_ex_return_def]
-  \\ every_case_tac \\ gs []
+  simp [dest_numeral_def, raise_Failure_def, st_ex_return_def]
+  \\ strip_tac
+  \\ rpt CASE_TAC \\ gs []
+  \\ rw [SF SFY_ss]
 QED
 
 Theorem num2bit_thm:
-  numeral_thy_ok (sigof ctxt, axsof ctxt) ⇒
+  numeral_thy_ok (thyof ctxt) ⇒
     TERM ctxt (num2bit x)
 Proof
   strip_tac \\ qid_spec_tac ‘x’
+  \\ drule_then strip_assume_tac numeral_thy_ok_terms_ok
   \\ ho_match_mp_tac num2bit_ind \\ rw []
   \\ gs [numeral_thy_ok_def]
   \\ rw [Once num2bit_def] \\ gs []
   \\ fs [TERM_def] \\ simp [Once term_ok_def]
+QED
+
+Theorem dest_num_num2bit:
+  numeral_thy_ok thy ⇒
+  ∀x y.
+    dest_num x = SOME y ⇒
+      (thy,[]) |- num2bit y === x
+Proof
+  strip_tac
+  \\ drule_then strip_assume_tac numeral_thy_ok_terms_ok
+  \\ ‘theory_ok thy’
+    by fs [numeral_thy_ok_def]
+  \\ ho_match_mp_tac dest_num_ind \\ rw []
+  \\ qpat_x_assum ‘dest_num _ = _’ mp_tac
+  \\ simp [Once dest_num_def]
+  \\ rw [CaseEqs ["term", "option", "bool"]]
+  \\ simp [Once num2bit_def, proves_REFL] \\ gs []
+  >- (
+    IF_CASES_TAC \\ gs []
+    >- (
+      gs [Once num2bit_def, numeral_thy_ok_def]
+      \\ cheat (* _0 === r ⇒ _0 === _BIT0 r *)
+    )
+    >- (
+      cheat (* proves_MK_COMB *)
+      )
+  )
+  \\ cheat (* proves_MK_COMB *)
+QED
+
+Theorem num2bit_dest_numeral:
+  dest_numeral (_NUMERAL x) s = (M_success y, s') ∧
+  numeral_thy_ok (thyof s.the_context) ⇒
+          s = s' ∧ (thyof s.the_context,[]) |- num2bit y === x
+Proof
+  simp [dest_numeral_def, st_ex_return_def, raise_Failure_def]
+  \\ CASE_TAC \\ gs [] \\ rw []
+  \\ drule_all dest_num_num2bit \\ rw []
+QED
+
+Theorem init_thm:
+  init ths ∧
+  EVERY (THM ctxt) ths ⇒
+    EVERY (THM ctxt) num_thms
+Proof
+  rw [init_def, EVERY_MEM]
+QED
+
+Theorem init_thy_ok:
+  init ths ∧
+  STATE ctxt s ∧
+  EVERY (THM ctxt) ths ⇒
+    numeral_thy_ok (thyof ctxt) ∧
+    bool_thy_ok (thyof ctxt)
+Proof
+  strip_tac
+  \\ drule_all_then assume_tac init_thm
+  \\ gs [num_thms_def, numeral_thy_ok_def, bool_thy_ok_def, STATE_def,
+         CONTEXT_def, THM_def, extends_theory_ok, init_theory_ok, SF SFY_ss]
 QED
 
 Theorem compute_add_thm:
@@ -139,8 +204,12 @@ Theorem compute_add_thm:
 Proof
   simp [compute_add_def, raise_Failure_def]
   \\ IF_CASES_TAC \\ gs [] \\ strip_tac
+  \\ drule_all_then strip_assume_tac init_thy_ok
+  \\ drule_then strip_assume_tac numeral_thy_ok_terms_ok
   \\ simp [Once st_ex_bind_def, otherwise_def]
   \\ CASE_TAC \\ gs []
+  \\ ‘TERM ctxt _ADD_TM’
+    by gs [TERM_def]
   \\ drule_all_then strip_assume_tac dest_binary_thm \\ gvs []
   \\ CASE_TAC \\ gs []
   \\ pairarg_tac \\ gvs []
@@ -149,39 +218,42 @@ Proof
   \\ CASE_TAC \\ gs []
   \\ simp [Once st_ex_bind_def] \\ CASE_TAC \\ gs []
   \\ drule_all_then strip_assume_tac dest_numeral_thm \\ gvs []
-  \\ CASE_TAC \\ gs []
-  \\ simp [Once st_ex_bind_def] \\ CASE_TAC \\ gs []
-  \\ drule_then (qspec_then ‘ctxt’ mp_tac) mk_eq_thm \\ gs []
-  \\ impl_keep_tac
-  >- (
-    irule num2bit_thm
-    \\ cheat (* init ths and EVERY (THM ctxt) ths means numeral_thy_ok.
-                probably.
-              *))
-  \\ strip_tac \\ gvs []
-  \\ rename [‘num2bit (x + y)’, ‘dest_binary _ _ s = (M_success(l,r), _)’]
-  \\ CASE_TAC \\ fs [st_ex_return_def]
+  \\ CASE_TAC \\ gvs []
+  \\ simp [Once st_ex_bind_def, st_ex_return_def] \\ CASE_TAC \\ gs []
+  \\ rename [‘num2bit (x + y)’,
+             ‘dest_binary _ (_ADD (_NUMERAL l) (_NUMERAL r)) s’]
+  \\ ‘TERM ctxt (_NUMERAL (num2bit (x + y)))’
+    by (‘TERM ctxt (num2bit (x + y))’
+          suffices_by rw [TERM_def, term_ok_def]
+        \\ simp [num2bit_thm])
+  \\ drule_then (qspec_then ‘ctxt’ mp_tac) mk_eq_thm
+  \\ impl_tac >- fs []
+  \\ strip_tac \\ rveq
+  \\ CASE_TAC \\ fs []
   \\ rw [] \\ rw [THM_def]
-  \\ ‘tm = _ADD l r’
-    by (qpat_x_assum ‘dest_binary _ tm _ = _’ mp_tac
-        \\ simp [dest_binary_def, raise_Failure_def, st_ex_return_def]
-        \\ CASE_TAC \\ gs []
-        \\ CASE_TAC \\ gs []
-        \\ CASE_TAC \\ gs []
-        \\ IF_CASES_TAC \\ gs [] \\ rw []
-        \\ cheat (* The term tm isn't type checked, but it contains a constant
-                    named «+» and they have to have the same type. *))
-  \\ gvs []
-  \\ ‘term_type (_ADD l r) = num_ty’
+  \\ ‘term_type (_ADD (_NUMERAL l) (_NUMERAL r)) = num_ty’
     by (fs [STATE_def]
         \\ qpat_x_assum ‘TERM _ (_ADD _ _)’ assume_tac
         \\ drule_all term_type \\ gs [])
   \\ gvs []
-  \\ ‘l = num2bit x ∧ r = num2bit y’
-    by cheat (* Theorem relating dest_numeral and num2bit *)
-  \\ gs []
-  \\ irule (SIMP_RULE (srw_ss()) [equation_def] ADD_num2bit)
-  \\ cheat (* numeral_thy_ok again *)
+  \\ ‘(thyof ctxt,[]) |- _NUMERAL l === num2bit x ∧
+      (thyof ctxt,[]) |- _NUMERAL r === num2bit y’
+    by (‘(thyof ctxt,[]) |- l === num2bit x ∧ (thyof ctxt,[]) |- r === num2bit y’
+          suffices_by cheat (* TODO trans *)
+        \\ gs [num2bit_dest_numeral, STATE_def, sym_equation])
+  \\ ‘(thyof ctxt,[]) |- _ADD (_NUMERAL l) (_NUMERAL r) ===
+                         _NUMERAL (num2bit (x + y))’
+    suffices_by rw [equation_def]
+  \\ ‘(thyof ctxt,[]) |- _ADD (num2bit x) (_NUMERAL r) ===
+                         _NUMERAL (num2bit (x + y))’
+    suffices_by cheat (* TODO replacement *)
+  \\ ‘(thyof ctxt,[]) |- _ADD (num2bit x) (num2bit y) ===
+                         _NUMERAL (num2bit (x + y))’
+    suffices_by cheat (* TODO replacement *)
+  \\ ‘(thyof ctxt,[]) |- _ADD (num2bit x) (num2bit y) ===
+                         num2bit (x + y)’
+    suffices_by cheat (* TODO replacement, _NUMERAL x === x *)
+  \\ irule ADD_num2bit \\ gs []
 QED
 
 val _ = export_theory ();
